Add files via upload

EBPFSpec/Instructions.lean
@@ -6,36 +6,30 @@ import EBPFSpec.Memory
 -------------------------------------------------
 
 inductive opCode where
-  | add_K_32 (dst : Reg) (imm : ℕ )
-  | add_X_32 (dst src : Reg)
-  | and_K_32 (dst : Reg) (imm : ℕ )
-  | and_X_32 (dst src : Reg)
+  | add_K (dst : Reg) (imm : ℕ )
+  | add_X (dst src : Reg)
+  | and_K (dst : Reg) (imm : ℕ )
+  | and_X (dst src : Reg)
   --| add_K_64 (dst : Reg) (imm : ℕ )
   --| add_X_64 (dst src : Reg)
-  | mov_K_32 (dst : Reg) (imm : ℕ )
-  | mov_X_32 (dst src : Reg)
+  | mov_K (dst : Reg) (imm : ℕ )
+  | mov_X (dst src : Reg)
   --| jmp_K_32 (offset : ℕ )
   --| jmp_X_32 (offset : ℕ )
-  | jgt_K_32 (dst : Reg) (imm : ℕ ) (offset : ℕ )
-  | jgt_X_32 (dst src : Reg) (offset : ℕ )
-  | jne_K_32 (dst : Reg) (imm : ℕ ) (offset : ℕ )
-  | jne_X_32 (dst src : Reg) (offset : ℕ )
-  | jeq_K_32 (dst : Reg) (imm : ℕ ) (offset : ℕ )
-  | jeq_X_32 (dst src : Reg) (offset : ℕ )
-  | jset_K_32 (dst : Reg) (imm : ℕ ) (offset : ℕ )
-  | jset_X_32 (dst src : Reg) (offset : ℕ )
+  | jgt_K (dst : Reg) (imm : ℕ ) (offset : ℕ )
+  | jgt_X (dst src : Reg) (offset : ℕ )
+  | jne_K (dst : Reg) (imm : ℕ ) (offset : ℕ )
+  | jne_X (dst src : Reg) (offset : ℕ )
+  | jeq_K (dst : Reg) (imm : ℕ ) (offset : ℕ )
+  | jeq_X (dst src : Reg) (offset : ℕ )
+  | jset_K (dst : Reg) (imm : ℕ ) (offset : ℕ )
+  | jset_X (dst src : Reg) (offset : ℕ )
   --| ldh_K_32 (imm : ℕ ) (index : ℕ )
-  | ldh_X_32 (dst : Reg) (src : Reg) (index : ℕ )
+  | ldh_X (dst : Reg) (src : Reg) (index : ℕ )
   --| ldxh_K_32 (imm : ℕ ) (index : ℕ )
-  | ldxh_X_32 (dst : Reg) (index : ℕ )
-  | sth_K_32 (imm index : ℕ )
-  | sth_X_32 (src : Reg) (index : ℕ )
+  --| ldxh_X (dst : Reg) (index : ℕ )
+  | sth_K (imm index : ℕ )
+  | sth_X (src : Reg) (index : ℕ )
   | exit
-
--- (ℕ → ℕ → Prop)
-
-/-
-Qual o tipos do operadores <,>,=, criar uma classe JMP operador reg reg offset
--/
 
 abbrev Code := List opCode
